fmi/fmi_export.thy
@@ -1,0 +1,14 @@
+(******************************************************************************)
+(* Project: The Isabelle/UTP Proof System                                     *)
+(* File: fmi_export.thy                                                       *)
+(* Authors: Frank Zeyda and Simon Foster (University of York, UK)             *)
+(* Emails: frank.zeyda@york.ac.uk and simon.foster@york.ac.uk                 *)
+(******************************************************************************)
+(* LAST REVIEWED: 8 Feb 2017 *)
+
+section {* FMI {\Circus} Model *}
+
+theory fmi_export
+imports fmi
+begin
+end
